proof/correctness/easycrypt_extra/List_extra.ec
@@ -1,6 +1,6 @@
 require import AllCore StdOrder List Ring IntDiv.
 (*---*) import IntOrder.
-require import Ring_extra.
+require import Ring_extra IntDiv_extra.
 
 
 (*-----------------------------------------------------------------------------*)
@@ -26,6 +26,129 @@ proof.
 qed.
 
 
+(*-----------------------------------------------------------------------------*)
+
+
+(*TODO: why is it not using left_commutative? Modify.*)
+print foldr_perm.
+
+op left_commutative_in ['b 'a] o (z : 'b) (s : 'a list) =
+  forall x y ,
+    x \in s =>
+    y \in s =>
+    o x (o y z) = o y (o x z).
+
+lemma foldr_perm_in ['b 'a] o (s1 s2 : 'a list) :
+  (forall (z : 'b) , left_commutative_in o z s1) =>
+  perm_eq s1 s2 =>
+  (forall (z : 'b) , foldr o z s1 = foldr o z s2).
+proof.
+  elim: s1 s2 => [|h1 t1 IHs1] s2 Hlci Heqs12 /=.
+  + by have -> //: s2 = []; apply/perm_eq_small/perm_eq_sym.
+  have/perm_eq_mem/(_ h1) := Heqs12; rewrite mem_head /=.
+  move/splitPr => [h2 t2] ->> z; rewrite foldr_cat /=.
+  move: Heqs12; rewrite -(cat1s h1 t2) catA perm_eq_sym.
+  rewrite perm_catCA /= perm_cons perm_eq_sym => Heqs1_.
+  move: (IHs1 _ _ Heqs1_); first by move => w a b Has1 Hbs1; apply/Hlci => /=; right.
+  move => ->; rewrite foldr_cat; have Heqin:= (perm_eq_mem _ _ Heqs1_).
+  have {Heqs1_ Heqin Hlci} Hlci: forall z , left_commutative_in o z (h1 :: h2).
+  + by move => w a b /= [->>|Hat1] [->>|Hbt2]; apply/Hlci => //=; right; rewrite Heqin mem_cat; left.
+  elim: h2 Hlci => [|x h2 {IHs1} IHs1 Hlci] //=.
+  rewrite -IHs1; first by move => w a b /= [->>|Has1] [->>|Hbs1] //; apply/Hlci => //=; rewrite ?Has1 ?Hbs1.
+  by rewrite Hlci.
+qed.
+
+
+(*-----------------------------------------------------------------------------*)
+
+search _ (_ \in range _ _).
+
+(*TODO: why must I specify the type int here?*)
+lemma mem_range_incl (m1 n1 m2 n2 i : int) :
+  m2 <= m1 =>
+  n1 <= n2 =>
+  i \in range m1 n1 =>
+  i \in range m2 n2.
+proof. by rewrite !mem_range => ? ? [? ?]; split;[apply/(lez_trans m1)|move => _; apply/(ltr_le_trans n1)]. qed.
+
+lemma mem_range_addl (m n x y : int) :
+  x + y \in range m n <=> y \in range (m - x) (n - x).
+proof. by rewrite !mem_range ler_subl_addl ltr_subr_addl. qed.
+
+lemma mem_range_addr (m n x y : int) :
+  x + y \in range m n <=> x \in range (m - y) (n - y).
+proof. by rewrite addrC mem_range_addl. qed.
+
+lemma mem_range_add2 (m1 n1 m2 n2 x y : int) :
+  x \in range m1 n1 =>
+  y \in range m2 n2 =>
+  x + y \in range (m1 + m2) (n1 + n2 - 1).
+proof. by rewrite !mem_range => -[? ?] [? ?]; rewrite ler_add //= ltr_subr_addl addrA ler_lt_add // lez_add1r. qed.
+
+lemma mem_range_opp (m n x : int) :
+  -x \in range m n <=> x \in range (- n + 1) (- m + 1).
+proof. by rewrite !mem_range -ltzE ltzS ler_oppr ltr_oppl. qed.
+
+lemma mem_range_subl (m n x y : int) :
+  x - y \in range m n <=> y \in range (- n + x + 1) (- m + x + 1).
+proof. by rewrite mem_range_addl mem_range_opp !opprD. qed.
+
+lemma mem_range_subr (m n x y : int) :
+  x - y \in range m n <=> x \in range (m + y) (n + y).
+proof. by rewrite mem_range_addr. qed.
+
+lemma mem_range_mull (m n x y : int) :
+  0 < x =>
+  x * y \in range m n <=> y \in range (m %\ x) (n %\ x).
+proof. by move => lt0x; rewrite !mem_range lez_NdivNRL // ltz_NdivNLR // !(mulrC y). qed.
+
+lemma mem_range_mulr (m n x y : int) :
+  0 < y =>
+  x * y \in range m n <=> x \in range (m %\ y) (n %\ y).
+proof. by rewrite mulrC; apply/mem_range_mull. qed.
+
+lemma mem_range_mul (m1 n1 m2 n2 x y : int) :
+  0 <= m1 =>
+  0 <= m2 =>
+  x \in range m1 n1 =>
+  y \in range m2 n2 =>
+  x * y \in range (m1 * m2) (n1 * n2 - n1 - n2 + 2).
+proof.
+  rewrite !mem_range => le0m1 le0m2 [lem1x ltxn1] [lem2x ltn2]; split; first by apply ler_pmul.
+  move => _; rewrite ltzE -ler_subr_addr /=; move: (ler_pmul x (n1 - 1) y (n2 - 1)).
+  by rewrite mulrDl !mulrDr mulNr mulrN /= !addrA => -> //;
+  [apply/(lez_trans m1)|apply/(lez_trans m2)|apply/ltzS|apply/ltzS].
+qed.
+
+lemma mem_range_add_mul (m n l x y : int) :
+  x \in range 0 l =>
+  y \in range m n =>
+  x + l * y \in range (m * l) (n * l).
+proof.
+  move => Hx_range Hy_range; rewrite mem_range_addl mem_range_mull; first by apply/(ler_lt_trans x); move/mem_range: Hx_range.
+  move: Hy_range; apply/mem_range_incl.
+  + rewrite lez_NdivNRL; first by apply/(ler_lt_trans x); move/mem_range: Hx_range.
+    by rewrite ler_subl_addr ler_addl; move/mem_range: Hx_range.
+  rewrite -ltzS -ltr_subl_addr ltz_NdivNLR; first by apply/(ler_lt_trans x); move/mem_range: Hx_range.
+  by rewrite mulrDl mulNr /= ler_lt_sub //; move/mem_range: Hx_range.
+qed.
+
+lemma mem_range_add_mul_eq (x1 y1 x2 y2 l : int) :
+  x1 \in range 0 l =>
+  x2 \in range 0 l =>
+  x1 + l * y1 = x2 + l * y2 <=>
+  x1 = x2 /\ y1 = y2.
+proof.
+  move => /mem_range [le0x1 ltx1l] /mem_range [le0x2 ltx2l]; split => [Heq|[->> ->>] //]; split.
+  + move: (congr1 (transpose (%%)%IntID l) _ _ Heq) => /=.
+    by rewrite !(mulrC l) !modzMDr !pmod_small.
+  move: (congr1 (transpose (%/)%IntID l) _ _ Heq) => /=.
+  rewrite !(mulrC l) !divzMDr; try by apply/gtr_eqF/(ler_lt_trans x1).
+  by rewrite !pdiv_small.
+qed.
+
+
+(*TODO: remove all lemmas below.*)
 (*-----------------------------------------------------------------------------*)
 
 lemma range_incl (x min1 max1 min2 max2 : int) :
